Simplify Reg, Opcode, Format

RV32I/Def.lean
@@ -12,214 +12,101 @@ The [ascii doc source](https://github.com/riscv/riscv-isa-manual/blob/main/src/r
 /-! ## 2.1. Programmers' Model for Base Integer ISA
 -/
 
-inductive Reg
-  /-- Zero. Immutable. -/
-  | zero
-  /-- Return address. -/
-  | ra
-  /-- Stack pointer. Preserved across calls. -/
-  | sp
-  /-- Global pointer. Unallocatable. -/
-  | gp
-  /-- Thread pointer. Unallocatable. -/
-  | tp
-  /-- Temporary registers. -/
-  | t (i : Fin 7)
-  /-- Callee-saved registers. Preserved across calls. -/
-  | s (i : Fin 12)
-  /-- Argument registers. -/
-  | a (i : Fin 8)
+abbrev Reg := BitVec 5
+namespace Reg
 
-instance Reg.x : Equiv (Fin 32) Reg where
-  toFun
-  := ![
+/-- Zero. Immutable. -/
+def zero : Reg := 0
+/-- Return address. -/
+def ra : Reg := 1
+/-- Stack pointer. Preserved across calls. -/
+def sp : Reg := 2
+/-- Global pointer. Unallocatable. -/
+def gp : Reg := 3
+/-- Thread pointer. Unallocatable. -/
+def tp : Reg := 4
+/-- Temporary registers. -/
+def t : Fin 7 → Reg := ![5, 6, 7, 28, 29, 30, 31]
+/-- Callee-saved registers. Preserved across calls. -/
+def s : Fin 12 → Reg := ![8, 9, 18, 19, 20, 21, 22, 23, 24, 25, 26, 27]
+/-- Argument registers. -/
+def a : Fin 8 → Reg := ![10, 11, 12, 13, 14, 15, 16, 17]
+
+def x : Fin 32 → Reg := ![
     zero, ra, sp, gp, tp, t 0, t 1, t 2,
     s 0, s 1, a 0, a 1, a 2, a 3, a 4, a 5,
     a 6, a 7, s 2, s 3, s 4, s 5, s 6, s 7,
     s 8, s 9, s 10, s 11, t 3, t 4, t 5, t 6
   ]
-    -- | 0 => zero | 1 => ra | 2 => sp | 3 => gp | 4 => tp
-    -- | 5 => t 0 | 6 => t 1 | 7 => t 2
-    -- | 8 => s 0 | 9 => s 1
-    -- | 10 => a 0 | 11 => a 1 | 12 => a 2 | 13 => a 3 | 14 => a 4 | 15 => a 5
-    --   | 16 => a 6 | 17 => a 7
-    -- | 18 => s 2 | 19 => s 3 | 20 => s 4 | 21 => s 5 | 22 => s 6 | 23 => s 7
-    --   | 24 => s 8 | 25 => s 9 | 26 => s 10 | 27 => s 11
-    -- | 28 => t 3 | 29 => t 4 | 30 => t 5 | 31 => t 6
-    -- | ⟨n + 32, (h : n + 32 < 32)⟩ =>
-    --   absurd (Nat.le_add_left 32 n) (Nat.not_le_of_gt h)
-  invFun
-    | zero => 0 | ra => 1 | sp => 2 | gp => 3 | tp => 4
-    | t 0 => 5 | t 1 => 6 | t 2 => 7
-    | s 0 => 8 | s 1 => 9
-    | a ⟨n, _⟩ => n + 10
-    | s ⟨n + 2, _⟩ => n + 18
-    -- | t 3 => 28 | t 4 => 29 | t 5 => 30 | t 6 => 31
-    | t ⟨n + 3, _⟩ => n + 28
-  left_inv (i : Fin 32) := by fin_cases i <;> rfl
-  right_inv (x : Reg) := by
-    cases x <;> try rfl
-    case t i => fin_cases i <;> rfl
-    case s i => fin_cases i <;> rfl
-    case a i => fin_cases i <;> rfl
 
-instance : Coe Reg (BitVec 5) where
-  coe x := Reg.x.symm x
+example (i : Fin 32) : x i = i := by fin_cases i <;> rfl
 
-instance : Coe (BitVec 5) Reg where
-  coe i := Reg.x i.toFin
+end Reg
+
+namespace Inst
 
 /-- Table 70. RISC-V base opcode map, `inst[1:0]=11`. -/
-inductive Opcode : Type
-  -- `inst[6:5]=00`
-  | LOAD | «LOAD-FP» | «custom-0» | «MISC-MEM» | «OP-IMM» | AUIPC | «OP-IMM-32» | «48b»
-  -- `inst[6:5]=01`
-  | STORE | «STORE-FP» | «custom-1» | AMO | OP | LUI | «OP-32» | «64b»
-  -- `inst[6:5]=10`
-  | MADD | MSUB | NMSUB | NMADD | «OP-FP» | «OP-V» | «custom-2/rv128»
-    /-- Rewritten as `48b` in the spec. -/ | «48b'»
-  -- `inst[6:5]=11`
-  | BRANCH | JALR | reserved | JAL | SYSTEM | «OP-VE» | «custom-3/rv128» | «≥80b»
+abbrev Opcode := BitVec 7
+namespace Opcode
 
-def Opcode.toBitVec : Opcode → BitVec 7
-  -- `inst[6:5]=00`
-  | LOAD             => 0b00_000_11
-  | «LOAD-FP»        => 0b00_001_11
-  | «custom-0»       => 0b00_010_11
-  | «MISC-MEM»       => 0b00_011_11
-  | «OP-IMM»         => 0b00_100_11
-  | AUIPC            => 0b00_101_11
-  | «OP-IMM-32»      => 0b00_110_11
-  | «48b»            => 0b00_111_11
-  -- `inst[6:5]=01`
-  | STORE            => 0b01_000_11
-  | «STORE-FP»       => 0b01_001_11
-  | «custom-1»       => 0b01_010_11
-  | AMO              => 0b01_011_11
-  | OP               => 0b01_100_11
-  | LUI              => 0b01_101_11
-  | «OP-32»          => 0b01_110_11
-  | «64b»            => 0b01_111_11
-  -- `inst[6:5]=10`
-  | MADD             => 0b10_000_11
-  | MSUB             => 0b10_001_11
-  | NMSUB            => 0b10_010_11
-  | NMADD            => 0b10_011_11
-  | «OP-FP»          => 0b10_100_11
-  | «OP-V»           => 0b10_101_11
-  | «custom-2/rv128» => 0b10_110_11
-  | «48b'»           => 0b10_111_11
-  -- `inst[6:5]=11`
-  | BRANCH           => 0b11_000_11
-  | JALR             => 0b11_001_11
-  | reserved         => 0b11_010_11
-  | JAL              => 0b11_011_11
-  | SYSTEM           => 0b11_100_11
-  | «OP-VE»          => 0b11_101_11
-  | «custom-3/rv128» => 0b11_110_11
-  | «≥80b»           => 0b11_111_11
+def LOAD       : Opcode := 0b00_000_11
+def «MISC-MEM» : Opcode := 0b00_011_11
+def «OP-IMM»   : Opcode := 0b00_100_11
+def AUIPC      : Opcode := 0b00_101_11
+def STORE      : Opcode := 0b01_000_11
+def AMO        : Opcode := 0b01_011_11
+def OP         : Opcode := 0b01_100_11
+def LUI        : Opcode := 0b01_101_11
+def BRANCH     : Opcode := 0b11_000_11
+def JALR       : Opcode := 0b11_001_11
+def JAL        : Opcode := 0b11_011_11
+def SYSTEM     : Opcode := 0b11_100_11
 
-instance : Coe Opcode (BitVec 7) where
-  coe := Opcode.toBitVec
+end Opcode
 
-theorem Opcode.toBitVec_lsbs_all_one (opcode : Opcode)
-  : opcode.toBitVec.extractLsb 1 0 = 0b11#2 := by cases opcode <;> trivial
+/-! ## 2.2. Base Instruction Formats
+-/
 
-/-- 2.2. Base Instruction Formats -/
-class inductive Inst.Format
-  | Rtype
-    : (funct7       : BitVec  7)
-    → (rs2          : BitVec  5)
-    → (rs1          : BitVec  5)
-    → (funct3       : BitVec  3)
-    → (rd           : BitVec  5)
-    → Opcode → Format
-  | Itype
-    : («imm[11:0]»  : BitVec 12)
-    → (rs1          : BitVec  5)
-    → (funct3       : BitVec  3)
-    → (rd           : BitVec  5)
-    → Opcode → Format
-  | Stype
-    : («imm[11:5]»  : BitVec  7)
-    → (rs2          : BitVec  5)
-    → (rs1          : BitVec  5)
-    → (funct3       : BitVec  3)
-    → («imm[4:0]»   : BitVec  5)
-    → Opcode → Format
-  | Btype
-    : («imm[12]»    : BitVec  1)
-    → («imm[10:5]»  : BitVec  6)
-    → (rs2          : BitVec  5)
-    → (rs1          : BitVec  5)
-    → (funct3       : BitVec  3)
-    → («imm[4:1]»   : BitVec  4)
-    → («imm[11]»    : BitVec  1)
-    → Opcode → Format
-  | Utype
-    : («imm[31:12]» : BitVec 20)
-    → (rd           : BitVec  5)
-    → Opcode → Format
-  | Jtype
-    : («imm[20]»    : BitVec  1)
-    → («imm[10:1]»  : BitVec 10)
-    → («imm[11]»    : BitVec  1)
-    → («imm[19:12]» : BitVec  8)
-    → (rd           : BitVec  5)
-    → Opcode → Format
+def Utype («imm[31:12]» : BitVec 20) (rd : BitVec 5) (opcode : Opcode) : UInt32 :=
+  UInt32.mk («imm[31:12]» ++ rd ++ opcode)
 
-namespace Inst.Format
+def Itype («imm[11:0]» : BitVec 12) (rs1 : BitVec 5) (funct3 : BitVec 3) rd opcode :=
+  Utype («imm[11:0]» ++ rs1 ++ funct3) rd opcode
+
+/-- `pred,succ = iorw` -/
+abbrev Mtype (fm pred succ : BitVec 4) rs1 funct3 rd :=
+  Itype (fm ++ pred ++ succ) rs1 funct3 rd .«MISC-MEM»
+
+def Rtype (funct7 : BitVec 7) (rs2 : BitVec 5) rs1 funct3 rd opcode :=
+  Itype (funct7 ++ rs2) rs1 funct3 rd opcode
 
 abbrev Rtype' funct7 rs2 rs1 funct3 rd :=
   Rtype funct7 rs2 rs1 funct3 rd .OP
 
-/-- Shifts by a constant -/
-abbrev Itype' (funct7 : BitVec 7) (shamt : BitVec 5) rs1 funct3 rd :=
-  Itype (funct7 ++ shamt) rs1 funct3 rd .«OP-IMM»
+/-- Shift by a constant. A variant of I-type. -/
+abbrev Itype' funct7 shamt rs1 funct3 rd :=
+  Rtype funct7 shamt rs1 funct3 rd .«OP-IMM»
 
-/-- `pred,succ = iorw` -/
-abbrev Mtype (fm pred succ : BitVec  4) rs1 funct3 rd :=
-  Itype (fm ++ pred ++ succ) rs1 funct3 rd .«MISC-MEM»
+def Stype (offset : BitVec 12) rs2 rs1 funct3 :=
+  let «imm[11:5]» : BitVec 7 := offset.extractLsb 11 5
+  let «imm[4:0]»  : BitVec 5 := offset.extractLsb  4 0
+  Rtype «imm[11:5]» rs2 rs1 funct3 «imm[4:0]» .STORE
 
-abbrev Stype' (offset : BitVec 12) rs2 rs1 funct3 :=
-  Stype
-    (offset.extractLsb 11 5)
-    rs2 rs1 funct3
-    (offset.extractLsb  4 0)
-    .STORE
+def Btype (offset1 : BitVec 12) rs2 rs1 funct3 :=
+  let «imm[12]»   : BitVec 1 := offset1.extractLsb 11 11
+  let «imm[10:5]» : BitVec 6 := offset1.extractLsb  9  4
+  let «imm[4:1]»  : BitVec 4 := offset1.extractLsb  3  0
+  let «imm[11]»   : BitVec 1 := offset1.extractLsb 10 10
+  Rtype («imm[12]» ++ «imm[10:5]») rs2 rs1 funct3 («imm[4:1]» ++ «imm[11]») .BRANCH
 
-abbrev Btype' (offset1 : BitVec 12) rs2 rs1 funct3 :=
-  Btype
-    (offset1.extractLsb 11 11)
-    (offset1.extractLsb  9  4)
-    rs2 rs1 funct3
-    (offset1.extractLsb  3  0)
-    (offset1.extractLsb 10 10)
-    .BRANCH
+def Jtype (offset1 : BitVec 20) rd :=
+  let «imm[20]»    : BitVec  1 := offset1.extractLsb 19 19
+  let «imm[10:1]»  : BitVec 10 := offset1.extractLsb  9  0
+  let «imm[11]»    : BitVec  1 := offset1.extractLsb 10 10
+  let «imm[19:12]» : BitVec  8 := offset1.extractLsb 18 11
+  Utype («imm[20]» ++ «imm[10:1]» ++ «imm[11]» ++ «imm[19:12]») rd .JAL
 
-abbrev Jtype' (offset1 : BitVec 20) rd :=
-  Jtype
-    (offset1.extractLsb 19 19)
-    (offset1.extractLsb  9  0)
-    (offset1.extractLsb 10 10)
-    (offset1.extractLsb 18 11)
-    rd .JAL
-
-def toUInt32 : Format → UInt32
-  | Rtype funct7 rs2 rs1 funct3 rd opcode =>
-    UInt32.mk <| funct7 ++ rs2 ++ rs1 ++ funct3 ++ rd ++ opcode.toBitVec
-  | Itype «imm[11:0]» rs1 funct3 rd opcode =>
-    UInt32.mk <| «imm[11:0]» ++ rs1 ++ funct3 ++ rd ++ opcode.toBitVec
-  | Stype «imm[11:5]» rs2 rs1 funct3 «imm[4:0]» opcode =>
-    UInt32.mk <| «imm[11:5]» ++ rs2 ++ rs1 ++ funct3 ++ «imm[4:0]» ++ opcode.toBitVec
-  | Btype «imm[12]» «imm[10:5]» rs2 rs1 funct3 «imm[4:1|11]» «imm[11]» opcode =>
-    UInt32.mk <| «imm[12]» ++ «imm[10:5]» ++ rs2 ++ rs1 ++ funct3 ++ «imm[4:1|11]» ++ «imm[11]» ++ opcode.toBitVec
-  | Utype «imm[31:12]» rd opcode =>
-    UInt32.mk <| «imm[31:12]» ++ rd ++ opcode.toBitVec
-  | Jtype «imm[20]» «imm[10:1]» «imm[11]» «imm[19:12]» rd opcode =>
-    UInt32.mk <| «imm[20]» ++ «imm[10:1]» ++ «imm[11]» ++ «imm[19:12]» ++ rd ++ opcode.toBitVec
-
-end Inst.Format
+end Inst
 
 /-! ## 2.4. Integer Computational Instructions
 
@@ -278,57 +165,55 @@ inductive Inst
 
 namespace Inst
 
-instance toFormat : Inst → Format
+def toUInt32 : Inst → UInt32
   /- 2.4.1. Integer Register-Immediate Instructions -/
-  | ADDI  rd  rs1 imm    => .Itype  imm          rs1 0b000 rd .«OP-IMM»
-  | SLTI  rd  rs1 imm    => .Itype  imm          rs1 0b010 rd .«OP-IMM»
-  | SLTIU rd  rs1 imm    => .Itype  imm          rs1 0b011 rd .«OP-IMM»
-  | ANDI  rd  rs1 imm    => .Itype  imm          rs1 0b111 rd .«OP-IMM»
-  | ORI   rd  rs1 imm    => .Itype  imm          rs1 0b110 rd .«OP-IMM»
-  | XORI  rd  rs1 imm    => .Itype  imm          rs1 0b100 rd .«OP-IMM»
-  | SLLI  rd  rs1 shamt  => .Itype'      0 shamt rs1 0b001 rd
-  | SRLI  rd  rs1 shamt  => .Itype'      0 shamt rs1 0b101 rd
-  | SRAI  rd  rs1 shamt  => .Itype'     32 shamt rs1 0b101 rd
-  | LUI   rd      imm    => .Utype  imm                    rd .LUI
-  | AUIPC rd      imm    => .Utype  imm                    rd .AUIPC
+  | ADDI  rd  rs1 imm    => Itype  imm          rs1 0b000 rd .«OP-IMM»
+  | SLTI  rd  rs1 imm    => Itype  imm          rs1 0b010 rd .«OP-IMM»
+  | SLTIU rd  rs1 imm    => Itype  imm          rs1 0b011 rd .«OP-IMM»
+  | ANDI  rd  rs1 imm    => Itype  imm          rs1 0b111 rd .«OP-IMM»
+  | ORI   rd  rs1 imm    => Itype  imm          rs1 0b110 rd .«OP-IMM»
+  | XORI  rd  rs1 imm    => Itype  imm          rs1 0b100 rd .«OP-IMM»
+  | SLLI  rd  rs1 shamt  => Itype'      0 shamt rs1 0b001 rd
+  | SRLI  rd  rs1 shamt  => Itype'      0 shamt rs1 0b101 rd
+  | SRAI  rd  rs1 shamt  => Itype'     32 shamt rs1 0b101 rd
+  | LUI   rd      imm    => Utype  imm                    rd .LUI
+  | AUIPC rd      imm    => Utype  imm                    rd .AUIPC
   /- 2.4.2. Integer Register-Register Operations -/
-  | ADD   rd  rs1 rs2    => .Rtype'      0 rs2   rs1 0b000 rd
-  | SLT   rd  rs1 rs2    => .Rtype'      0 rs2   rs1 0b010 rd
-  | SLTU  rd  rs1 rs2    => .Rtype'      0 rs2   rs1 0b011 rd
-  | AND   rd  rs1 rs2    => .Rtype'      0 rs2   rs1 0b111 rd
-  | OR    rd  rs1 rs2    => .Rtype'      0 rs2   rs1 0b110 rd
-  | XOR   rd  rs1 rs2    => .Rtype'      0 rs2   rs1 0b100 rd
-  | SLL   rd  rs1 rs2    => .Rtype'      0 rs2   rs1 0b001 rd
-  | SRL   rd  rs1 rs2    => .Rtype'      0 rs2   rs1 0b101 rd
-  | SUB   rd  rs1 rs2    => .Rtype'     32 rs2   rs1 0b000 rd
-  | SRA   rd  rs1 rs2    => .Rtype'     32 rs2   rs1 0b101 rd
+  | ADD   rd  rs1 rs2    => Rtype'      0 rs2   rs1 0b000 rd
+  | SLT   rd  rs1 rs2    => Rtype'      0 rs2   rs1 0b010 rd
+  | SLTU  rd  rs1 rs2    => Rtype'      0 rs2   rs1 0b011 rd
+  | AND   rd  rs1 rs2    => Rtype'      0 rs2   rs1 0b111 rd
+  | OR    rd  rs1 rs2    => Rtype'      0 rs2   rs1 0b110 rd
+  | XOR   rd  rs1 rs2    => Rtype'      0 rs2   rs1 0b100 rd
+  | SLL   rd  rs1 rs2    => Rtype'      0 rs2   rs1 0b001 rd
+  | SRL   rd  rs1 rs2    => Rtype'      0 rs2   rs1 0b101 rd
+  | SUB   rd  rs1 rs2    => Rtype'     32 rs2   rs1 0b000 rd
+  | SRA   rd  rs1 rs2    => Rtype'     32 rs2   rs1 0b101 rd
   /- 2.5.1. Unconditional Jumps -/
-  | JAL   rd      offset => .Jtype' offset                 rd
-  | JALR  rd  rs1 offset => .Itype  offset       rs1 0b000 rd .JALR
+  | JAL   rd      offset => Jtype  offset                 rd
+  | JALR  rd  rs1 offset => Itype  offset       rs1 0b000 rd .JALR
   /- 2.5.2. Conditional Branches -/
-  | BEQ   rs1 rs2 offset => .Btype' offset rs2   rs1 0b000
-  | BNE   rs1 rs2 offset => .Btype' offset rs2   rs1 0b001
-  | BLT   rs1 rs2 offset => .Btype' offset rs2   rs1 0b100
-  | BGE   rs1 rs2 offset => .Btype' offset rs2   rs1 0b101
-  | BLTU  rs1 rs2 offset => .Btype' offset rs2   rs1 0b110
-  | BGEU  rs1 rs2 offset => .Btype' offset rs2   rs1 0b111
+  | BEQ   rs1 rs2 offset => Btype  offset rs2   rs1 0b000
+  | BNE   rs1 rs2 offset => Btype  offset rs2   rs1 0b001
+  | BLT   rs1 rs2 offset => Btype  offset rs2   rs1 0b100
+  | BGE   rs1 rs2 offset => Btype  offset rs2   rs1 0b101
+  | BLTU  rs1 rs2 offset => Btype  offset rs2   rs1 0b110
+  | BGEU  rs1 rs2 offset => Btype  offset rs2   rs1 0b111
   /- 2.6. Load and Store Instructions -/
-  | LW    rd  rs1 offset => .Itype  offset       rs1 0b010 rd .LOAD
-  | LH    rd  rs1 offset => .Itype  offset       rs1 0b001 rd .LOAD
-  | LHU   rd  rs1 offset => .Itype  offset       rs1 0b101 rd .LOAD
-  | LB    rd  rs1 offset => .Itype  offset       rs1 0b000 rd .LOAD
-  | LBU   rd  rs1 offset => .Itype  offset       rs1 0b100 rd .LOAD
-  | SW    rs2 rs1 offset => .Stype' offset rs2   rs1 0b010
-  | SH    rs2 rs1 offset => .Stype' offset rs2   rs1 0b001
-  | SB    rs2 rs1 offset => .Stype' offset rs2   rs1 0b000
+  | LW    rd  rs1 offset => Itype  offset       rs1 0b010 rd .LOAD
+  | LH    rd  rs1 offset => Itype  offset       rs1 0b001 rd .LOAD
+  | LHU   rd  rs1 offset => Itype  offset       rs1 0b101 rd .LOAD
+  | LB    rd  rs1 offset => Itype  offset       rs1 0b000 rd .LOAD
+  | LBU   rd  rs1 offset => Itype  offset       rs1 0b100 rd .LOAD
+  | SW    rs2 rs1 offset => Stype  offset rs2   rs1 0b010
+  | SH    rs2 rs1 offset => Stype  offset rs2   rs1 0b001
+  | SB    rs2 rs1 offset => Stype  offset rs2   rs1 0b000
   /- 2.7. Memory Ordering Instructions -/
-  | FENCE pred succ      => .Mtype 0 pred   succ   0 0b000  0
-  | FENCE.TSO            => .Mtype 8 0b0011 0b0011 0 0b000  0
+  | FENCE pred succ      => Mtype 0 pred   succ   0 0b000  0
+  | FENCE.TSO            => Mtype 8 0b0011 0b0011 0 0b000  0
   /- 2.8. Environment Call and Breakpoints -/
-  | ECALL                => .Itype              0  0 0b000  0 .SYSTEM
-  | EBREAK               => .Itype              1  0 0b000  0 .SYSTEM
-
-abbrev toUInt32 (inst : Inst) : UInt32 := inst.toFormat.toUInt32
+  | ECALL                => Itype              0  0 0b000  0 .SYSTEM
+  | EBREAK               => Itype              1  0 0b000  0 .SYSTEM
 
 namespace Pseudo
 
@@ -339,20 +224,20 @@ abbrev SEQZ rd rs1 := SLTIU rd rs1 1
 /-- `rd = ~~~rs1` -/
 abbrev NOT rd rs1 := XORI rd rs1 (-1 : Int)
 /-- `rd = if rs2 ≠ 0 then 1 else 0` -/
-abbrev SNEZ rd rs2 := SLTU rd .zero rs2
+abbrev SNEZ rd rs2 := SLTU rd 0 rs2
 /-- 2.4.3. NOP Instruction -/
-abbrev NOP := ADDI .zero .zero 0
+abbrev NOP := ADDI 0 0 0
 /-- Unconditional jump -/
-abbrev J offset := JAL .zero offset
+abbrev J offset := JAL 0 offset
 
 end Pseudo
 
 namespace Hint
 
-abbrev NTL.P1   := ADD .zero .zero (.x 2)
-abbrev NTL.PALL := ADD .zero .zero (.x 3)
-abbrev NTL.S1   := ADD .zero .zero (.x 4)
-abbrev NTL.ALL  := ADD .zero .zero (.x 5)
+abbrev NTL.P1   := ADD 0 0 2
+abbrev NTL.PALL := ADD 0 0 3
+abbrev NTL.S1   := ADD 0 0 4
+abbrev NTL.ALL  := ADD 0 0 5
 abbrev PAUSE    := FENCE 0b0001 0b0000
 
 end Hint
